implement typing for bil

bil_valuesScript.sml
@@ -109,36 +109,28 @@ val type_of_bil_val_def = Define `
   (type_of_bil_val (Imm imm) = SOME (ImmType (type_of_bil_imm imm))) /\
   (type_of_bil_val (Mem at vt _) = SOME (MemType at vt))`;
 
-val bil_type_is_NoType_def = Define `bil_type_is_NoType tyo = (tyo = NONE)`
-val bil_type_is_ImmType_def = Define `bil_type_is_ImmType tyo = (?s. tyo = SOME (ImmType s))`
-val bil_type_is_ImmType_s_def = Define `bil_type_is_ImmType_s s tyo = (tyo = SOME (ImmType s))`
-val bil_type_is_BoolType_def = Define `bil_type_is_BoolType tyo = (tyo = SOME (ImmType Bit1))`
-val bil_type_is_MemType_def = Define `bil_type_is_MemType tyo = (?at vt. tyo = SOME (MemType at vt))`;
+val bil_type_is_ImmType_def = Define `bil_type_is_ImmType ty = (?s. ty = ImmType s)`;
+val bil_type_is_ImmType_s_def = Define `bil_type_is_ImmType_s s ty = (ty = ImmType s)`
+val bil_type_is_BoolType_def = Define `bil_type_is_BoolType ty = (ty = ImmType Bit1)`
+val bil_type_is_MemType_def = Define `bil_type_is_MemType ty = (?at vt. ty = MemType at vt)`;
 
 val bil_type_checker_DEFS = save_thm ("bil_type_checker_DEFS", LIST_CONJ [
-  bil_type_is_NoType_def, bil_type_is_ImmType_def, bil_type_is_ImmType_s_def,
+  bil_type_is_ImmType_def, bil_type_is_ImmType_s_def,
   bil_type_is_BoolType_def, bil_type_is_MemType_def]);
 
 
-val bil_type_checker_REWRS = store_thm ("bil_type_checker_REWRS",
-  ``bil_type_is_NoType NONE /\
-    (!ty. ~bil_type_is_NoType (SOME ty)) /\
+val bil_type_checker_REWRS = store_thm ("bil_type_checker_REWRS", ``
+    (!b. bil_type_is_ImmType (ImmType b)) /\
+    (!at vt. ~(bil_type_is_ImmType (MemType at vt))) /\
 
-    ~(bil_type_is_ImmType NONE) /\
-    (!b. bil_type_is_ImmType (SOME (ImmType b))) /\
-    (!at vt. ~(bil_type_is_ImmType (SOME (MemType at vt)))) /\
+    (!b. ~(bil_type_is_MemType (ImmType b))) /\
+    (!at vt. (bil_type_is_MemType (MemType at vt))) /\
 
-    ~(bil_type_is_MemType NONE) /\
-    (!b. ~(bil_type_is_MemType (SOME (ImmType b)))) /\
-    (!at vt. (bil_type_is_MemType (SOME (MemType at vt)))) /\
+    (!s b. bil_type_is_ImmType_s s (ImmType b) <=> (b = s)) /\
+    (!s at vt. ~(bil_type_is_ImmType_s s (MemType at vt))) /\
 
-    (!s. ~(bil_type_is_ImmType_s s NONE)) /\
-    (!s b. bil_type_is_ImmType_s s (SOME (ImmType b)) <=> (b = s)) /\
-    (!s at vt. ~(bil_type_is_ImmType_s s (SOME (MemType at vt)))) /\
-
-    (~(bil_type_is_BoolType NONE)) /\
-    (!b. bil_type_is_BoolType (SOME (ImmType b)) <=> (b = Bit1)) /\
-    (!at vt. ~(bil_type_is_BoolType (SOME (MemType at vt))))``,
+    (!b. bil_type_is_BoolType (ImmType b) <=> (b = Bit1)) /\
+    (!at vt. ~(bil_type_is_BoolType (MemType at vt)))``,
 
   SIMP_TAC (std_ss ++ bil_type_ss) [bil_type_checker_DEFS]);
 
@@ -153,20 +145,15 @@ val bil_type_is_BoolType_IMPL = store_thm ("bil_type_is_BoolType_IMPL",
 SIMP_TAC (std_ss++bil_type_ss) [bil_type_is_ImmType_def, bil_type_is_BoolType_def]);
 
 
-val bil_type_check_bil_type_of_bil_val = store_thm ("bil_type_check_bil_type_of_bil_val",
-  ``(!v. (bil_type_is_NoType (type_of_bil_val v) <=> bil_val_is_Unknown v)) /\
-
-    (!v. (bil_type_is_ImmType (type_of_bil_val v) <=> bil_val_is_Imm v)) /\
-    (!v s. (bil_type_is_ImmType_s s (type_of_bil_val v) <=> bil_val_is_Imm_s s v)) /\
-    (!v. (bil_type_is_BoolType (type_of_bil_val v) <=> bil_val_is_Bool v)) /\
-    (!v. (bil_type_is_MemType (type_of_bil_val v) <=> bil_val_is_Mem v))``,
-
-REPEAT STRIP_TAC >> Cases_on `v` >> (
-  SIMP_TAC std_ss [bil_val_checker_REWRS, bil_type_checker_REWRS,
-    type_of_bil_val_def]
+val type_of_bil_val_EQ_ELIMS = store_thm ("type_of_bil_val_EQ_ELIMS",
+  ``(!v. (type_of_bil_val v = NONE) <=> (v = Unknown)) /\
+    (!v ty. (type_of_bil_val v = SOME (ImmType ty)) <=>
+            (?i. (type_of_bil_imm i = ty) /\ (v = Imm i))) /\
+    (!v aty vty. (type_of_bil_val v = SOME (MemType aty vty)) <=>
+            (?f. (v = Mem aty vty f)))``,
+REPEAT CONJ_TAC >> Cases >> (
+  SIMP_TAC (std_ss++bil_val_ss++bil_type_ss) [type_of_bil_val_def]
 ));
-
-
 
 
 val _ = export_theory();
